theories/System/STLC.v
@@ -9,4 +9,47 @@ Module ChurchStyleSTLC.
 
 Export ChurchStyleStlc.
 
+Notation "Gamma '∋' x '⦂' A" := (Lookup x A Gamma) : type_scope.
+Notation "Gamma '⊢' M '⦂' A" := (Typing Gamma M A) : type_scope.
+Notation "Gamma '⊢' M '=' N '⦂' A" := (equality Gamma M N A) : type_scope.
+Notation "Gamma '⊢' M '⇉' A" := (typNe Gamma M A) : type_scope.
+Notation "Gamma '⊢' M '⇇' A" := (typNf Gamma M A) : type_scope.
+
+Section STLC_META.
+
+Context {L : language}.
+
+Section KripkeLogicalRelation.
+
+Context {Sigma : signature L}.
+
+Lemma Typing_weakening {Gamma : ctx L} {Delta : ctx L} {e : trm L} {ty : typ L}
+  (TYPING : Typing Gamma e ty)
+  (LE : le_ctx Gamma Delta)
+  : Typing Delta e ty.
+Proof.
+  revert Delta LE. induction TYPING; simpl; intros.
+  - econs 1. eapply LE. exact LOOKUP.
+  - econs 2; eauto.
+  - econs 3; eapply IHTYPING. intros x ty LOOKUP. pattern LOOKUP. revert LOOKUP. eapply Lookup_cons.
+    + intros x_EQ ty_EQ. subst x ty. econs 1; reflexivity.
+    + intros x_NE LOOKUP. econs 2; eauto.
+  - econs 4.
+Defined.
+
+Definition substTyping (Gamma : ctx L) (s : subst L) (Delta : ctx L) : Set :=
+  forall x : name, forall ty : typ L, Lookup x ty Delta -> Typing Gamma (s x) ty.
+
+Lemma substTyping_Lookup {Gamma : ctx L} {x : Name.t} {ty : typ L} {s : subst L} {Delta : ctx L}
+  (LOOKUP : Gamma ∋ x ⦂ ty)
+  (SUBST_TYPING : substTyping Delta s Gamma)
+  : Delta ⊢ s x ⦂ ty.
+Proof.
+  eapply SUBST_TYPING; exact LOOKUP.
+Defined.
+
+End KripkeLogicalRelation.
+
+End STLC_META.
+
 End ChurchStyleSTLC.
